%! Author = francis
%! Date = 13.08.20

% Preamble
\documentclass[11pt, leqno]{article}

% Packages
\usepackage{amsfonts}
\usepackage{amssymb}
\usepackage{amsmath}

\usepackage{hyperref}

%\newcommand\numberthis{\addtocounter{equation}{1}\tag{\theequation}}
\numberwithin{equation}{section}
% Document
\begin{document}
    \section{Step by step derivation of $F_{R^h}$}\label{sec:steps}
Transformation of CDF:
    \begin{align}
        F_{-Y}(y)
        &= \mathbb{P}(-Y \leq y) \nonumber\\
        &= \mathbb{P}(Y \geq -y) \nonumber\\
        &= 1 - \mathbb{P}(Y \leq -y)\nonumber\\
        &= 1 - F_{Y}(-y)   \label{eq:tCDF}
    \end{align}
Transformation of Copula:
    \begin{align}
        C_{X,-Y}(u,v) &=
        F_{X,-Y}(F_X^{-1}(u),F_{-Y}^{-1}(v)) &&\text{Sklar}\nonumber\\
        &=
        \mathbb{P}(X \leq F_X^{-1}(u), -Y \leq F_{-Y}^{-1}(v)) \nonumber\\
        &=
        \mathbb{P}(F_X(X) \leq u, F_{-Y}(-Y) \leq v) \nonumber\\
        &=
        \mathbb{P}(F_X(X) \leq u, 1-F_{Y}(Y) \leq v) && \text{\eqref{eq:tCDF}}\nonumber\\
        &=
        \mathbb{P}(F_X(X) \leq u, F_{Y}(Y) \geq 1-v) \nonumber\\
        &=
        \mathbb{P}(X \leq F_X^{-1}(u), Y \geq F_Y^{-1}(1-v)) \nonumber\\
        &=
        F_X[F_X^{-1}(u)] - F_{X,Y}[F_X^{-1}(u), F_Y^{-1}(1-v)] \nonumber\\
        &=
        u - C_{X,Y}(u, 1-v) &&\text{Sklar} \label{eq:trans-Copula}
    \end{align}

We continue with the result from \eqref{eq:trans-Copula}:
    \begin{align}
        C_{X,-Y}(u,v) &= u - C_{X,Y}(u, 1-v)\nonumber\\
        \frac{\partial C_{X,-Y}(u,v)}{\partial u} &= 1 - \frac{\partial C_{X,Y}(u, 1-v)}{\partial u}\\
        \int^1_0 D_1 C_{X,-Y}(u,v)du &= 1 - \int^1_0 D_1 C_{X,Y}(u,1-v)du \label{eq:D1C_integral}
    \end{align}

Now we plug \eqref{eq:tCDF} and \eqref{eq:D1C_integral} into C-Convolution equation:
    \begin{align*}
        F_{R^h}(r^h) &= \int^1_0 D_1 C_{R^S, -hR^F}
        \{w,
        F_{-hR^F}[r^h - F^{-1}_{R^S}(w)
        ]\}dw \\
        &= 1 - \int^1_0 D_1C^t_{R^S, hR^F}
        \{w,
        1- F_{-hR^F}[r^h - F^{-1}_{R^S}(w)
        ]\}dw && \text{\eqref{eq:D1C_integral}}\\
        &= 1 - \int^1_0 D_1C^t_{R^S, hR^F}
        \{w,
        F_{hR^F}[F^{-1}_{R^S}(w) - r^h
        ]\}dw && \text{\eqref{eq:tCDF}}
    \end{align*}

We proceed wih $F_{hR^F}(x)=F_{R^F}(x/h)$ and $C_{R^S,hR^F}(w, \lambda)=C_{R^S,R^F}(w, \lambda)$:
    \begin{align*}
        F_{R^h}(r^h)
        &= 1- \int^1_0 D_1 C_{R^S, R^F}
        \left\{
        w,
        F_{R^F}
        \left[
        \frac{F^{-1}_{R^S}(w)-r^h}{h}
        \right]
        \right\}dw \\
    \end{align*}
Barbi and Romagnoli's proof of Corollary 2:
    \begin{align*}
        F_{R^h}(r^h)
        &= 1 - \int^1_0 D_1 C_{R^S, R^F}
        \left\{w,
        1- F_{hR^F}\left[\frac{r^h - F^{-1}_{R^S}(w)}{h}
        \right]\right\}dw \\
    \end{align*}
\end{document}